lab3 done

src/Lab3/LogImpl.v
@@ -69,7 +69,16 @@ Theorem diskGet_eq_values : forall d a b b',
     b = b'.
 Proof.
   (* Fill in your proof here. *)
-Admitted.
+  intros.
+  destruct (diskGet d a) eqn:Heq.
+  {
+    simpl in *.
+    subst; auto.
+  }
+  {
+    apply disk_inbounds_not_none in H1; auto.
+  }
+  Qed.
 
 (** We use the above theorem to implement the [eq_values]
     tactic.  [eq_values] can be used when you have hypotheses
@@ -97,19 +106,1099 @@ Module Log (d : OneDiskAPI) <: LogAPI.
       procedures and helper theorems to structure your implementation
       and proof. *)
 
-  Definition init : proc InitResult := Ret Initialized.
-  Definition get : proc (list block) := Ret nil.
-  Definition append (bs : list block) : proc bool := Ret true.
-  Definition reset : proc unit := Ret tt.
-  Definition recover : proc unit := Ret tt.
+  Set Nested Proofs Allowed.
 
-  Axiom abstr : Abstraction State.
-  Axiom init_ok : init_abstraction init recover abstr inited_any.
-  Axiom get_ok : proc_spec get_spec get recover abstr.
-  Axiom append_ok : forall v, proc_spec (append_spec v) (append v) recover abstr.
-  Axiom reset_ok : proc_spec reset_spec reset recover abstr.
-  Axiom recover_wipe : rec_wipe recover abstr no_wipe.
+  (** helper tactics *)
+  Ltac unfold_diskGet :=
+    match goal with
+    | [ |- context[diskGet ?l ?n] ] =>
+      replace (diskGet l n) with (nth_error l n) by auto; simpl
+    end.
 
+  Ltac fold_diskGet :=
+    match goal with
+    | [ |- context[nth_error ?l ?n] ] =>
+      replace (nth_error l n) with (diskGet l n) by auto; simpl
+    end.
+
+  Ltac unfold_diskSize :=
+    match goal with
+    | [ |- context[diskSize ?d] ] =>
+      replace (diskSize d) with (length d) by auto; simpl
+    end.
+
+  Ltac fold_diskSize :=
+    match goal with
+    | [ |- context[length ?d] ] =>
+      replace (length d) with (diskSize d) by auto; simpl
+    end.
+
+  (** helper definitions *)
+  Definition diskGetLogLength (d : disk) : nat :=
+    match diskGet d (diskSize d - 1) with
+    | Some v => block_to_addr v
+    | None => 0
+    end.
+
+  (** helper lemmas *)
+  Lemma diskGet_none_size:
+    forall d a,
+      diskGet d a = None -> ~(a < diskSize d).
+  Proof.
+    unfold not.
+    intros.
+    eapply disk_inbounds_not_none; eauto.
+  Qed.
+
+  Lemma diskGets_eq:
+    forall len d1 d2 a1 a2,
+      skipn a1 d1 = skipn a2 d2 ->
+      diskGets d1 a1 len = diskGets d2 a2 len.
+  Proof.
+    induction len.
+    1: auto.
+    intros.
+    pose H as H0.
+    eapply IHlen in H0.
+    replace (S len) with (len + 1) by lia.
+    do 2 rewrite diskGets_last.
+    assert (diskGet d1 (a1 + len) = diskGet d2 (a2 + len)).
+    {
+      do 2 unfold_diskGet.
+      Lemma nth_error_skipn:
+        forall (l: list block) a b,
+          nth_error l (a + b) = nth_error (skipn a l) b.
+      Proof.
+        induction l.
+        {
+          induction a.
+          1: auto.
+          intros.
+          simpl.
+          destruct b; auto.
+        }
+        {
+          intros.
+          simpl.
+          destruct a0.
+          1: auto.
+          simpl.
+          eapply IHl.
+        }
+      Qed.
+      do 2 rewrite nth_error_skipn.
+      rewrite H; auto.
+    }
+    rewrite H1.
+    rewrite H0.
+    reflexivity.
+  Qed.
+
+  (** abstraction relation *)
+  Inductive log_abstraction (disk_state : OneDiskAPI.State) (log_state : LogAPI.State) : Prop :=
+    | LogAbstraction :
+      let nonsense := 0 in
+      forall
+        (* maximum log length is (disk size - 1) *)
+        (Hlength_inbounds : ((not(diskSize disk_state = 0) -> length log_state < diskSize disk_state)) /\ (diskSize disk_state = 0 -> length log_state = 0))
+        (* last entry on disk is the same as log length (or log length is 0) *)
+        (Hlength_on_disk : length log_state = diskGetLogLength disk_state)
+        (* for all nats i below log length, the block at i on the disk corresponds to the block at i in the log. we use diskGets log_state here even though log_state isn't a disk to ease later
+         proofs. *)
+        (Hentries : diskGets log_state 0 (length log_state) = diskGets disk_state 0 (length log_state))
+      ,
+      log_abstraction disk_state log_state.
+  Definition abstr : Abstraction State :=
+    abstraction_compose d.abstr {| abstraction := log_abstraction |}.
+
+  (** recover function *)
+  Definition recover : proc unit := d.recover.
+  
+  Theorem recover_wipe : rec_wipe recover abstr no_wipe.
+  Proof.
+    unfold rec_wipe.
+    intros.
+
+    apply spec_abstraction_compose; simpl.
+    step_proc; eauto.
+  Qed.
+
+  (** init function *)
+  Definition init' : proc InitResult :=
+    sz <- d.size;
+    n_ <- addr_to_block 0;
+    _ <- d.write (sz - 1) n_;
+    Ret Initialized.
+  Definition init := then_init d.init init'.
+
+  Theorem init_ok : init_abstraction init recover abstr inited_any.
+  Proof.
+    eapply then_init_compose; eauto.
+    step_proc.
+    step_proc.
+    step_proc.
+    step_proc.
+    exists nil.
+    intuition.
+    constructor.
+    {
+      split.
+      {
+        intros.
+        simpl.
+        destruct state.
+        {
+          simpl in H0.
+          exfalso.
+          apply H0.
+          auto.
+        }
+        {
+          simpl.
+          destruct (diskSize state - 0); simpl; lia.
+        }
+      }
+      {
+        intros.
+        simpl.
+        auto.
+      }
+    }
+    {
+      simpl.
+      unfold diskGetLogLength.
+      destruct state.
+      {
+        simpl.
+        assert (diskGet nil 0 = None) by auto.
+        rewrite H0.
+        reflexivity.
+      }
+      {
+        simpl.
+        destruct (diskSize state - 0) eqn:Heq.
+        {
+          simpl.
+          rewrite Heq.
+          assert (diskGet (r :: state) 0 = Some r) by auto.
+          rewrite H0.
+          auto.
+        }
+        {
+          simpl.
+          rewrite diskUpd_size.
+          rewrite Heq.
+          unfold_diskGet.
+          fold_diskGet.
+          destruct (diskGet state n) eqn:Heq2.
+          {
+            SearchAbout (diskGet (diskUpd _ _ _) _).
+            eapply diskUpd_eq_some in Heq2.
+            instantiate (1:= r) in Heq2.
+            rewrite Heq2.
+            auto.
+          }
+          {
+            eapply diskGet_none_size in Heq2.
+            SearchAbout (diskGet (diskUpd _ _ _) _).
+            eapply diskUpd_oob_eq in Heq2.
+            instantiate (1:= r) in Heq2.
+            rewrite Heq2.
+            auto.
+          }
+        }
+      }
+    }
+    auto.
+  Qed.
+
+  (** get_log_length function (helper) *)
+  Definition get_log_length : proc nat :=
+    sz <- d.size;
+    if gt_dec sz 0 then
+      len <- d.read (sz - 1);
+      Ret (block_to_addr len)
+    else
+      Ret 0.
+
+  Definition get_log_length_spec : Specification unit nat unit OneDiskAPI.State :=
+    fun (_ : unit) state => {|
+        pre := True;
+        post := fun r state' =>
+                 state' = state /\
+                 r = diskGetLogLength state;
+        recovered := fun _ state' =>
+                      state' = state
+      |}.
+
+  Theorem get_log_length_ok : proc_spec get_log_length_spec get_log_length recover d.abstr.
+  Proof.
+    unfold get_log_length; intros.
+    step_proc.
+    destruct (gt_dec r 0).
+    {
+      step_proc.
+      step_proc.
+      unfold diskGetLogLength.
+      destruct state.
+      {
+        simpl in g.
+        lia.
+      }
+      {
+        SearchAbout (diskGet _ _ = Some _).
+        assert (exists r0, diskGet (b :: state) (diskSize (b :: state) - 1) = Some r0).
+        {
+          eapply disk_inbounds_exists.
+          lia.
+        }
+        destruct H0.
+        rewrite H0 in H1.
+        simpl in H1.
+        subst.
+        rewrite H0.
+        auto.
+      }
+    }
+    step_proc.
+    destruct state.
+    {
+      unfold diskGetLogLength.
+      unfold_diskGet.
+      auto.
+    }
+    {
+      exfalso.
+      apply n.
+      simpl.
+      lia.
+    }
+  Qed.
+
+  Hint Resolve get_log_length_ok : core.
+
+  (** get function *)
+  Fixpoint get_rec (len : nat) (remaining : nat) : proc (list block) :=
+    match remaining with
+    | 0 =>
+      Ret nil
+    | S remaining' =>
+      b <- d.read (len - (S remaining'));
+        rest <- get_rec len remaining';
+        Ret (b :: rest)
+    end.
+
+  Theorem get_rec_ok : forall (len:nat) (remaining:nat),
+      proc_spec (fun (_ : unit) disk_state => {|
+        pre := len <= diskSize disk_state /\ remaining <= len;
+        post := fun blocks disk_state' =>
+                 disk_state' = disk_state /\
+                 (* diskGets returns a list of options >:( *)
+                 map Some blocks = diskGets disk_state (len-remaining) (remaining)
+                 ;
+        recovered := fun _ disk_state' =>
+                      disk_state' = disk_state
+      |}) (get_rec len remaining) recover d.abstr.
+  Proof.
+    intros.
+    induction remaining.
+    {
+      simpl.
+      step_proc.
+    }
+    {
+      simpl.
+      step_proc.
+      step_proc.
+      1 : lia.
+      step_proc.
+      rewrite H3.
+      replace (len - S remaining + 1) with (len - remaining) by lia.
+      assert (Some r = diskGet state (len - S remaining)).
+      {
+        destruct (diskGet state (len - S remaining)) eqn:Heq.
+        {
+          simpl in H2.
+          subst; auto.
+        }
+        {
+          apply diskGet_none_size in Heq.
+          lia.
+        }
+      }
+      rewrite H1.
+      reflexivity.
+    }
+  Qed.
+
+  Hint Resolve get_rec_ok : core.
+
+  Definition get : proc (list block) :=
+    len <- get_log_length;
+    r <- get_rec len len;
+    Ret r.
+  
+  Theorem get_ok : proc_spec get_spec get recover abstr.
+  Proof.
+    unfold get.
+    apply spec_abstraction_compose; simpl.
+
+    step_proc.
+    {
+      exists state2.
+      intuition.
+    }
+    step_proc.
+    {
+      inversion H0.
+      destruct Hlength_inbounds.
+      rewrite <- Hlength_on_disk.
+      destruct (diskSize state) eqn:Heq.
+      {
+        intuition.
+        rewrite H2.
+        lia.
+      }
+      {
+        intuition.
+        lia.
+      }
+    }
+    {
+      exists state2.
+      intuition.
+    }
+    step_proc.
+    {
+      exists state2.
+      intuition.
+      inversion H0.
+      rewrite <- Hlength_on_disk in H2.
+      replace (length state2 - length state2) with 0 in H2 by lia.
+      rewrite <- H2 in Hentries.
+      clear - Hentries.
+      generalize dependent state2.
+      induction r; intros.
+      {
+        destruct state2.
+        1: auto.
+        simpl in *.
+        inversion Hentries.
+      }
+      {
+        destruct state2.
+        {
+          simpl in *.
+          inversion Hentries.
+        }
+        {
+          simpl in *.
+          inversion Hentries.
+          replace (diskGet (b :: state2) 0) with (Some b) in H0 by auto.
+          assert (diskGets (b :: state2) 1 (length state2) = diskGets state2 0 (length state2)).
+          {
+            eapply diskGets_eq.
+            auto.
+          }
+          intuition.
+          assert (r = state2).
+          {
+            eapply IHr.
+            rewrite <- H1.
+            auto.
+          }
+          subst; auto.
+        }
+      }
+    }
+    exists state2.
+    intuition.
+  Qed.
+  
+  (** append function *)
+  Fixpoint append_rec (bs : list block) (end' : nat) : proc unit :=
+    match bs with
+    | nil =>
+      Ret tt
+    | cons b bs' =>
+      _ <- d.write (end' - length bs) b;
+      _ <- append_rec bs' (end');
+      Ret tt
+    end.
+
+  Theorem append_rec_ok : forall (bs : list block) (end_ : nat) ,
+      proc_spec (fun (_ : unit) disk_state =>
+                   let len := diskGetLogLength disk_state in
+                   let addr := (end_ - length bs) in {|
+                     pre := end_ < (diskSize disk_state)
+                           /\ end_ > 0
+                           /\ length bs <= end_ - len;
+                     post := fun _ disk_state' =>
+                              disk_state' = diskUpds disk_state addr bs /\
+                              diskGetLogLength disk_state' = diskGetLogLength disk_state /\
+                              diskSize disk_state' = diskSize disk_state;
+                     recovered := fun _ disk_state' =>
+                                   disk_state' = disk_state \/
+                                   diskGets disk_state' 0 addr = diskGets disk_state 0 addr /\
+                                   diskGetLogLength disk_state = diskGetLogLength disk_state' /\
+
+                                   diskSize disk_state' = diskSize disk_state
+                                   ;
+      |}) (append_rec bs end_) recover d.abstr.
+  Proof.
+    induction bs.
+    {
+      simpl.
+      step_proc.
+      left; auto.
+    }
+    {
+      simpl.
+      step_proc.
+      {
+        destruct H2.
+        1: left; auto.
+        right.
+        split; intuition.
+        {
+          Lemma diskGets_upd_eq:
+            forall len d a b begin,
+              a >= begin + len ->
+              diskGets (diskUpd d a b) begin len = diskGets d begin len.
+          Proof.
+            induction len.
+            {
+              intros; simpl.
+              auto.
+            }
+            {
+              intros.
+              simpl.
+              specialize (IHlen d a b (begin + 1)).
+              assert (a >= begin + 1 + len) by lia.
+              intuition.
+              rewrite IHlen.
+              assert (diskGet d [a |-> b] begin = diskGet d begin).
+              {
+                eapply diskUpd_neq.
+                lia.
+              }
+              rewrite H1.
+              reflexivity.
+            }
+          Qed.
+          eapply diskGets_upd_eq.
+          lia.
+        }
+        {
+          unfold diskGetLogLength.
+          rewrite diskUpd_size.
+          assert (diskGet state (diskSize state - 1) = diskGet state [end_ - S (length bs) |-> a] (diskSize state - 1)).
+          {
+            symmetry.
+            eapply diskUpd_neq.
+            lia.
+          }
+          rewrite H2.
+          auto.
+        }
+        {
+          rewrite diskUpd_size.
+          auto.
+        }
+      }
+      step_proc.
+      {
+        rewrite diskUpd_size.
+        lia.
+      }
+      {
+        unfold diskGetLogLength.
+        rewrite diskUpd_size.
+        rewrite diskUpd_neq.
+        2: lia.
+        unfold diskGetLogLength in H1.
+        lia.
+      }
+      {
+        destruct H2.
+        {
+          right.
+          split.
+          {
+            subst.
+            apply diskGets_upd_eq.
+            lia.
+          }
+          split.
+          {
+            subst.
+            unfold diskGetLogLength.
+            rewrite diskUpd_size.
+            rewrite diskUpd_neq.
+            2: lia.
+            auto.
+          }
+          {
+            subst.
+            rewrite diskUpd_size.
+            auto.
+          }
+        }
+        {
+          destruct H2.
+          destruct H3.
+          right.
+          split.
+          {
+            Lemma diskGets_short:
+              forall len2 len1 d1 d2 a1 a2,
+                len1 <= len2 ->
+                diskGets d1 a1 len2 = diskGets d2 a2 len2 ->
+                diskGets d1 a1 len1 = diskGets d2 a2 len1.
+            Proof.
+              induction len2.
+              {
+                intros.
+                replace (len1) with 0 by lia.
+                auto.
+              }
+              {
+                intros.
+                simpl in H0.
+                inversion H0.
+                destruct len1.
+                1: auto.
+                simpl.
+                rewrite H2.
+                apply (IHlen2 len1) in H3.
+                2: lia.
+                rewrite H3.
+                auto.
+              }
+            Qed.
+            eapply diskGets_short in H2.
+            2: instantiate (1:= (end_ - S (length bs))); lia.
+            rewrite H2.
+            eapply diskGets_upd_eq.
+            lia.
+          }
+          split.
+          {
+            unfold diskGetLogLength in *.
+            rewrite diskUpd_size in H3.
+            rewrite diskUpd_neq in H3.
+            2: lia.
+            auto.
+          }
+          {
+            rewrite diskUpd_size in H4.
+            auto.
+          }
+        }
+      }
+      step_proc.
+      {
+        replace (end_ - S (length bs) + 1) with (end_ - length bs) by lia.
+        Lemma diskUpd_upds_comm:
+          forall bs a_sin a_list d b,
+            a_sin < a_list ->
+            d [a_sin |-> b] [a_list |=> bs] = d [a_list |=> bs] [a_sin |-> b].
+        Proof.
+          induction bs.
+          {
+            intros.
+            simpl.
+            auto.
+          }
+          {
+            intros.
+            destruct a_list.
+            1: lia.
+            simpl.
+            rewrite IHbs.
+            2: lia.
+            rewrite diskUpd_comm.
+            2: lia.
+            auto.
+          }
+        Qed.
+        rewrite diskUpd_upds_comm.
+        2: lia.
+        auto.
+      }
+      {
+        rewrite H3.
+        unfold diskGetLogLength.
+        rewrite diskUpd_size.
+        rewrite diskUpd_neq.
+        2: lia.
+        reflexivity.
+      }
+      {
+        rewrite H4.
+        rewrite diskUpd_size.
+        reflexivity.
+      }
+      right.
+      split.
+      {
+        rewrite diskUpd_upds_comm.
+        2: lia.
+        rewrite diskGets_upd_eq.
+        2: lia.
+        Lemma diskGets_upds_eq:
+          forall bs len d a begin,
+            a >= begin + len ->
+            diskGets (diskUpds d a bs) begin len = diskGets d begin len.
+        Proof.
+          induction bs.
+          1: auto.
+          intros.
+          destruct a0.
+          {
+            simpl.
+            replace len with 0 by lia.
+            auto.
+          }
+          {
+            simpl.
+            rewrite diskGets_upd_eq.
+            2: assumption.
+            eapply IHbs.
+            lia.
+          }
+        Qed.
+        rewrite diskGets_upds_eq.
+        2: lia.
+        auto.
+      }
+      split.
+      {
+        rewrite H3.
+        unfold diskGetLogLength.
+        rewrite diskUpd_size.
+        rewrite diskUpd_neq.
+        2: lia.
+        auto.
+      }
+      {
+        rewrite H4.
+        rewrite diskUpd_size.
+        auto.
+      }
+    }
+  Qed.
+
+  Hint Resolve append_rec_ok : core.
+
+  Definition append (bs : list block) : proc bool :=
+    size <- d.size;
+      len <- get_log_length;
+      if length bs == 0 then
+        Ret true
+      else if lt_dec (len + length bs) (size-1) then
+             _ <- append_rec bs (len + length bs);
+               new_len <- addr_to_block (len + length bs);
+               _ <- d.write (size - 1) new_len;
+               Ret true
+           else
+             Ret false.
+
+  Theorem append_ok : forall bs, proc_spec (append_spec bs) (append bs) recover abstr.
+  Proof.
+    intros.
+    apply spec_abstraction_compose; simpl.
+    step_proc.
+    {
+      exists state2.
+      intuition.
+    }
+    step_proc.
+    {
+      exists state2.
+      intuition.
+    }
+    destruct (equal_dec (length bs) 0).
+    {
+      step_proc.
+      {
+        exists (state2 ++ bs).
+        split.
+        1: left; auto.
+        destruct bs.
+        {
+          replace (state2 ++ []) with state2.
+          1: assumption.
+          SearchAbout (_ = _ ++ []).
+          apply app_nil_end.
+        }
+        {
+          simpl in *.
+          lia.
+        }
+      }
+      exists state2.
+      intuition.
+    }
+    {
+      destruct (lt_dec (r + length bs) (diskSize state - 1)).
+      {
+        step_proc; try lia.
+        {
+          destruct H1.
+          {
+            exists state2.
+            intuition.
+          }
+          {
+            destruct H1.
+            destruct H2.
+            inversion H0.
+            exists state2.
+            split.
+            1: intuition.
+            constructor.
+            1: split; intros; lia.
+            1: rewrite Hlength_on_disk; auto.
+            rewrite Hentries.
+            replace (diskGetLogLength state + length bs - length bs) with (diskGetLogLength state) in H1 by lia.
+            rewrite Hlength_on_disk.
+            auto.
+          }
+        }
+        assert (Hmodify: log_abstraction state [diskGetLogLength state |=> bs] state2).
+        {
+          inversion H0.
+          constructor.
+          {
+            split; intros.
+            1: rewrite diskUpds_size; lia.
+            intuition.
+            apply H3.
+            rewrite diskUpds_size in H1.
+            auto.
+          }
+          {
+            rewrite Hlength_on_disk.
+            Lemma diskGetLogLength_no_upds:
+              forall bs disk start,
+                start + length bs <= diskSize disk - 1 ->
+                diskGetLogLength (diskUpds disk start bs) = diskGetLogLength disk.
+            Proof.
+              induction bs.
+              1: auto.
+              intros.
+              destruct start.
+              {
+                simpl.
+                unfold diskGetLogLength in *.
+                rewrite diskUpd_size.
+                destruct disk.
+                1: simpl in H; lia.
+                destruct disk.
+                1: simpl in H; lia.
+                rewrite diskUpd_neq.
+                {
+                  rewrite IHbs.
+                  1: auto.
+                  simpl in *.
+                  auto.
+                }
+                rewrite diskUpds_size.
+                simpl.
+                auto.
+              }
+              {
+                simpl.
+                unfold diskGetLogLength in *.
+                rewrite diskUpd_size.
+                rewrite diskUpd_neq.
+                {
+                  rewrite IHbs.
+                  1: auto.
+                  simpl in *.
+                  lia.
+                }
+                simpl in *.
+                rewrite diskUpds_size.
+                lia.
+              }
+            Qed.
+            rewrite diskGetLogLength_no_upds.
+            1: auto.
+            lia.
+          }
+          rewrite diskGets_upds_eq.
+          1: auto.
+          lia.
+        }
+        assert (Hmodify2: forall r0,
+                   block_to_addr r0 = diskGetLogLength state + length bs ->
+                   log_abstraction state [diskGetLogLength state |=> bs] [diskSize state - 1 |-> r0] (state2 ++ bs)).
+        {
+          intros.
+          inversion H0.
+          constructor.
+          {
+            split; intros;
+              try rewrite diskUpd_size in *;
+              try rewrite diskUpds_size in *.
+            {
+              rewrite app_length.
+              lia.
+            }
+            intuition.
+            lia.
+          }
+          {
+            unfold diskGetLogLength.
+            rewrite diskUpd_size.
+            rewrite diskUpds_size.
+            rewrite diskUpd_eq.
+            {
+              rewrite app_length.
+              rewrite H1.
+              lia.
+            }
+            rewrite diskUpds_size.
+            destruct state; lia.
+          }
+          {
+            rewrite app_length.
+            rewrite diskUpd_diskGets_neq.
+            2: lia.
+            rewrite <- Hlength_on_disk in *.
+            repeat rewrite diskGets_app.
+            assert (diskGets (state2 ++ bs) 0 (length state2) = diskGets state [length state2 |=> bs] 0 (length state2)).
+            {
+              rewrite diskGets_upds_eq by lia.
+              rewrite <- Hentries.
+              destruct (length state2) eqn:Heq2.
+              1: auto.
+              rewrite <- Heq2 in *.
+              rewrite diskGets_app_disk.
+              2: lia.
+              {
+                replace (length state2 - 0) with (length state2) by lia.
+                replace (length state2 - length state2) with 0 by lia.
+                simpl.
+                apply app_nil_r.
+              }
+              lia.
+            }
+            rewrite H2.
+            simpl.
+            assert (diskGets state [length state2 |=> bs] (length state2) (length bs) = map Some bs).
+            {
+              eapply diskUpds_diskGets_eq.
+              lia.
+            }
+            rewrite H3.
+            Lemma diskGets_app_right:
+              forall b a,
+                diskGets (a ++ b) (length a) (length b) = map Some b.
+            Proof.
+              induction b.
+              1: auto.
+              simpl.
+              assert (forall l, diskGet (l ++ a :: b) (length l) = Some a).
+              {
+                induction l.
+                1: auto.
+                simpl.
+                unfold_diskGet.
+                auto.
+              }
+              intros.
+              rewrite H.
+              specialize (IHb (a0 ++ [a])).
+              rewrite app_length in IHb.
+              simpl in IHb.
+              assert ((a0 ++ [a]) ++ b = a0 ++ a :: b).
+              {
+                SearchAbout ((_ ++ _) ++ _).
+                rewrite <- app_assoc.
+                simpl.
+                auto.
+              }
+              rewrite <- H0.
+              rewrite IHb.
+              auto.
+            Qed.
+            rewrite diskGets_app_right.
+            auto.
+          }
+        }
+        step_proc.
+        {
+          exists state2.
+          intuition.
+          replace (diskGetLogLength state + length bs - length bs) with (diskGetLogLength state) by lia.
+          auto.
+        }
+        step_proc.
+        {
+          destruct H1.
+          {
+            exists state2.
+            intuition.
+            replace (diskGetLogLength state + length bs - length bs) with (diskGetLogLength state) by lia.
+            auto.
+          }
+          {
+            exists (state2 ++ bs).
+            intuition.
+            try replace (diskGetLogLength state + length bs - length bs) with (diskGetLogLength state) in * by lia.
+            intuition.
+          }
+        }
+        step_proc.
+        {
+          exists (state2 ++ bs).
+          intuition.
+          replace (diskGetLogLength state + length bs - length bs) with (diskGetLogLength state) by lia.
+          intuition.
+        }
+        exists (state2 ++ bs).
+        replace (diskGetLogLength state + length bs - length bs) with (diskGetLogLength state) by lia.
+        intuition.
+      }
+      step_proc.
+      {
+        exists state2.
+        intuition.
+      }
+      exists state2.
+      intuition.
+    }
+  Qed.
+
+  (** reset function *)
+  Definition reset : proc unit :=
+    sz <- d.size;
+      n_ <- addr_to_block 0;
+      _ <- d.write (sz - 1) n_;
+      Ret tt.
+  
+  Theorem reset_ok : proc_spec reset_spec reset recover abstr.
+  Proof.
+    unfold reset.
+    apply spec_abstraction_compose; simpl.
+    step_proc.
+    {
+      exists state2.
+      intuition.
+    }
+    step_proc.
+    {
+      exists state2.
+      intuition.
+    }
+    step_proc.
+    {
+      destruct H1.
+      {
+        exists state2.
+        intuition.
+      }
+      {
+        exists [].
+        intuition.
+        inversion H0.
+        constructor.
+        {
+          split; intros.
+          2: auto.
+          destruct (diskSize state [diskSize state - 1 |-> r]).
+          1: exfalso; apply H; auto.
+          simpl; lia.
+        }
+        {
+          simpl in *.
+          unfold diskGetLogLength in *.
+          rewrite diskUpd_size.
+          destruct state eqn:Heq.
+          {
+            simpl.
+            unfold_diskGet.
+            auto.
+          }
+          {
+            rewrite diskUpd_eq.
+            1: auto.
+            simpl.
+            lia.
+          }
+        }
+        {
+          simpl.
+          auto.
+        }
+      }
+    }
+    step_proc.
+    {
+      exists [].
+      intuition.
+      inversion H0.
+      constructor.
+      {
+        split; intros.
+        2: auto.
+        simpl; lia.
+      }
+      {
+        simpl.
+        unfold diskGetLogLength in *.
+        rewrite diskUpd_size.
+        destruct state eqn:Heq.
+        {
+          simpl.
+          unfold_diskGet.
+          auto.
+        }
+        {
+          rewrite diskUpd_eq.
+          1: auto.
+          simpl; lia.
+        }
+      }
+      {
+        auto.
+      }
+    }
+    exists [].
+    intuition.
+    inversion H0.
+    constructor.
+    {
+      split; intros.
+      2: auto.
+      simpl; lia.
+    }
+    {
+      simpl.
+      unfold diskGetLogLength in *.
+      rewrite diskUpd_size.
+      destruct state eqn:Heq.
+      {
+        simpl.
+        unfold_diskGet.
+        auto.
+      }
+      {
+        rewrite diskUpd_eq.
+        1: auto.
+        simpl; lia.
+      }
+    }
+    {
+      auto.
+    }
+  Qed.
+
+  Hint Resolve reset_ok : core.
 
 End Log.
 
